src/example/Client01.v
@@ -1,0 +1,148 @@
+From sflib Require Import sflib.
+From Paco Require Import paco.
+Require Import Coq.Classes.RelationClasses Lia Program.
+From Fairness Require Import pind Axioms ITreeLib Red TRed IRed2 WFLibLarge.
+From Fairness Require Import FairBeh Mod Concurrency Linking.
+From Fairness Require Import PCM IProp IPM IPropAux.
+From Fairness Require Import IndexedInvariants OpticsInterp SimWeakest.
+From Fairness Require Import TemporalLogic TemporalLogicFull SCMemSpec.
+
+Module Client01.
+
+  Definition gvs : list nat := [1].
+  Definition X := SCMem.val_ptr (0, 0).
+
+  Section CODE.
+
+    Notation state := unit.
+    Notation ident := void.
+
+    Definition thread1 :
+      ktree (threadE ident state) unit SCMem.val
+      :=
+      fun _ =>
+        `_ : unit <- (OMod.call "store" (X, 1));;
+        _ <- trigger Yield;;
+        Ret (0 : SCMem.val).
+
+    Definition thread2 :
+      ktree (threadE ident state) unit SCMem.val
+      :=
+      fun _ =>
+        _ <- trigger Yield;;
+        a <- (ITree.iter (fun (_ : unit) =>
+                           `a : SCMem.val <- (OMod.call "load" X);;
+                                `b : bool <- (OMod.call "compare" (a, 0));;
+                                     if b then Ret (inl tt) else Ret (inr a))) tt;;
+        _ <- trigger Yield;;
+        Ret a.
+
+    Definition omod : Mod.t :=
+      Mod.mk
+        tt
+        (Mod.get_funs [("thread1", Mod.wrap_fun thread1);
+                       ("thread2", Mod.wrap_fun thread2)])
+    .
+
+    Definition module : Mod.t :=
+      OMod.close
+        (omod)
+        (SCMem.mod gvs)
+    .
+
+  End CODE.
+
+End Client01.
+
+Module Client01Spec.
+
+  Section SPEC.
+
+    Notation state := unit.
+    Notation ident := void.
+
+    Definition thread1 :
+      ktree (threadE ident state) unit SCMem.val
+      :=
+      fun _ =>
+        _ <- trigger Yield;; Ret (0 : SCMem.val).
+
+    Definition thread2:
+      ktree (threadE void unit) unit SCMem.val
+      :=
+      fun _ =>
+        _ <- trigger Yield;; Ret (1 : SCMem.val).
+
+    Definition module : Mod.t :=
+      Mod.mk
+        tt
+        (Mod.get_funs [("thread1", Mod.wrap_fun thread1);
+                       ("thread2", Mod.wrap_fun thread2)])
+    .
+
+  End SPEC.
+
+End Client01Spec.
+
+Section SPEC.
+
+  Import Client01.
+
+  Notation src_state := (Mod.state Client01Spec.module).
+  Notation src_ident := (Mod.ident Client01Spec.module).
+  Notation tgt_state := (Mod.state Client01.module).
+  Notation tgt_ident := (Mod.ident Client01.module).
+
+  Local Instance STT : StateTypes := Build_StateTypes src_state tgt_state src_ident tgt_ident.
+  Context `{Σ : GRA.t}.
+  Context {TLRAS : @TLRAs XAtom STT Σ}.
+  Context {AUXRAS : AUXRAs Σ}.
+
+  (** Invariants. *)
+
+  (* Namespace for Client01 invariants. *)
+  Definition N_Client01 : namespace := (nroot .@ "Client01").
+  Definition N_t1_write : namespace := (nroot .@ "t1_write").
+
+  Lemma mask_disjoint_client01 : ↑N_Client01 ## (↑N_t1_write : coPset).
+  Proof. apply ndot_ne_disjoint. ss. Qed.
+
+  Definition t1_write n : Formula n :=
+    syn_inv n N_t1_write (X ↦ 1)%F.
+
+  Global Instance t1_write_persistent n : Persistent (⟦t1_write n, n⟧).
+  Proof.
+    unfold Persistent. iIntros "H". unfold t1_write. rewrite red_syn_inv.
+    iDestruct "H" as "#H". auto.
+  Qed.
+
+  Definition client01Inv k n : Formula n :=
+    ((◆[k, 2] ∗ -[k](0)-◇ t1_write n)
+      ∗
+      ((live[k] (1/2) ∗ (X ↦ 0))
+       ∨
+         (t1_write n))
+    )%F.
+
+  (* Simulation proof. *)
+
+  Lemma Client01_thread1_spec
+        tid n
+    :
+    ⊢ ⟦(∀ (k : τ{nat, 1+n}),
+           ((⤉ syn_inv n N_Client01 (client01Inv k n))
+              ∗ ○(tid) ∗ (⤉ Duty(tid) [(k, 0, t1_write n)]) ∗ ◇[k](1, 1) ∗ live[k] (1/2))
+             -∗
+             syn_wpsim (S n) tid ∅
+             (fun rs rt => ((⤉ syn_term n tid rs rt))%F : Formula (S n))
+             false false
+             (fn2th Client01Spec.module "thread1" (tt ↑))
+             (fn2th Client01.module "thread1" (tt ↑)))%F, 1+n⟧.
+  Proof.
+    iIntros. red_tl. iIntros (k). red_tl. simpl.
+    iEval (rewrite red_syn_inv; rewrite red_syn_wpsim).
+    iIntros "(#INV & THDW & DUTY & PCk)".
+
+  Admitted.
+
+End SPEC.
